fix type errors in concurrency-strategies/spec.s

examples/concurrency-strategies/spec.s.dfy
@@ -1,38 +1,56 @@
-type View = seq<nat>
-
-function LeastIndexOf(view:View, victim:nat) : (idx:Option<Nat>)
-  ensures forall j::0<=j<i ==> view[j] != victim
-  ensures i<|board| ==> view[i] == victim
-{
-...
-}
-
-function Donate(view:View, victim:nat) : (view':View, outidx: Option<nat>) {
-  outidx := LeastIndexOf(view, victim);
-  if idx.None? then
-    view' == view
-  else:
-    view' == view[idx.value := victim + 1]
-}
-
-
 module Abstract {
+  type View = seq<nat>
+  datatype Option<V> = None | Some(value:V)
+
+  datatype Op = DonateOp(victim:nat, outidx: Option<nat>)
+  type UI = Option<Op>
+
+  function LeastIndexOf(view:View, victim:nat) : (idx:Option<nat>)
+    ensures idx.None? ==> 
+      forall j | 0 <= j < |view| :: view[j] != victim
+    ensures idx.Some? ==>
+      && idx.value < |view|
+      && view[idx.value] == victim
+      && forall j | 0 <= j < idx.value :: view[j] != victim
+  {
+    if |view| == 0 then None else (
+      if view[0] == victim then Some(0) else (
+        var t := LeastIndexOf(view[1..], victim);
+        if t.Some? then (
+          Some(t.value + 1)
+        ) else (
+          None
+        )
+      )
+    )
+  }
+
+  function Donate(view:View, victim:nat, ui:UI) : (View, Option<nat>) {
+    var outidx := LeastIndexOf(view, victim);
+    var view' := (
+      if outidx.None? then
+        view
+      else
+        view[outidx.value := victim + 1]
+    );
+    (view', outidx)
+  }
 
   datatype State = State(board:View)
 
   predicate DonateStep(s:State, s':State, victim:nat, ui:UI) {
-    var view',outidx := Donate(s, victim);
-    && s' == view'
-    && ui == Some((victim, outidx))
+    var (view',outidx) := Donate(s.board, victim, ui);
+    && s' == State(view')
+    && ui == Some(DonateOp(victim, outidx))
   }
 
   predicate NoopStep(s:State, s':State) {
     s' == s
   }
 
-  predicate Next(s:State, s':State) {
-    || (exists victim, outidx :: DonateStep(s, s', victim, ui:UI)
-    || (NoopStep(s, s') && ui==None())
+  predicate Next(s:State, s':State, ui:UI) {
+    || (exists victim :: DonateStep(s, s', victim, ui))
+    || (NoopStep(s, s') && ui==None)
   }
 
 }
@@ -48,7 +66,7 @@ module Concrete {
 
   type Board = seq<Well>
 
-  datatype State = (board:Board, threads:set<Thread>)
+  datatype State = State(board:Board, threads:set<Thread>)
 
   function View(board:Board, i:nat) : (v:seq<nat>)
     ensures |v| == |board| - i
@@ -95,7 +113,7 @@ module Concrete {
       && ui == None()
     else
       // Need to advance, but waiting on a lock
-      && s' = s
+      && s' == s
       && ui == None()
   }
 
@@ -104,7 +122,7 @@ module Concrete {
     || Advance(s, s', ui)
   }
 
-  function I(s:State) : (as:Abstract.State) {
+  function I(s:State) : (abs:Abstract.State) {
     s.board[0].suffix
   }
 
